Move various utilities to coqutil

src/Utils/Eqb.v
@@ -1,41 +1,25 @@
-Set Implicit Arguments.
-
-(* TODO: add/cut dep on Booleans?
- TODO: leave instances here or move them?*)
-Require Coq.Bool.Bool.
-Require Import Utils.Base Datatypes.Bool Datatypes.String Lists.List Uint63.
-Import ListNotations.
+Require Import Utils.Base Datatypes.Bool Datatypes.String Uint63.
+Require Export coqutil.Eqb.
 
 
 Section __.
   Context (A : Type).
 
-  (* Not defined as a record so that firstorder doesn't mess with it*)
-  Definition Eqb := A -> A -> bool.
-  Definition eqb {Impl : Eqb} : A -> A -> bool := Impl.
-  Existing Class Eqb.
-
-  
-  (* Not defined as a record so that firstorder doesn't mess with it*)
-  Definition Eqb_ok `{Eqb} := forall a b, if eqb a b then a = b else a <> b.
-  Definition eqb_spec {Impl : Eqb} {Pf : @Eqb_ok Impl} : forall a b, if eqb a b then a = b else a <> b := Pf.
-  Existing Class Eqb_ok.
-
-  
   (* TODO: is the no-record version worth it here to avoid firstorder trouble? *)
   Class DecidableEq :=
     {
       dec : forall (s1 s2 : A), {s1 = s2} + {s1 <> s2}
     }.
 
-  (* Note: do not export. Should be declared as an instance only when no boolean implementation yet exists
-     since it will likely have poor performance.   
+  Context `{DecidableEq}.
+  
+  (* Note: do not export. Should be declared as an instance only when no boolean implementation yet exists since it will likely have poor performance.   
    *)
-  Instance eqb_from_decidable `{DecidableEq} : Eqb :=
+  Instance eqb_from_decidable : Eqb A :=
     fun a b => if dec a b then true else false.
 
   
-  Instance eqb_from_decidable_ok `{DecidableEq} : Eqb_ok.
+  Instance eqb_from_decidable_ok `{DecidableEq} : Eqb_ok eqb_from_decidable.
   Proof.
     intros a b.
     unfold eqb, eqb_from_decidable.
@@ -43,7 +27,7 @@ Section __.
   Qed.
 
 
-  Context `{Eqb_ok}.
+  Context `{@Eqb_ok _ eqb_from_decidable}.
   
   (* Note: do not export. This instance should not be expected to compute, since it depends on a lemma
      that is probably defined with Qed. To emphasize this, we define this instance with Qed as well.
@@ -55,105 +39,14 @@ Section __.
     specialize (H0 s1 s2).
     revert H0.
     case_match;
-      basic_goal_prep;
-      basic_utils_crush.
+      intros; subst; eauto.
   Qed.
 
-
-  Lemma eqb_prop_iff
-    : forall a b, Is_true (eqb a b) <-> a = b.
-  Proof.
-    intros a b.
-    specialize (H0 a b); revert H0.
-    case_match;
-      basic_goal_prep;
-      basic_utils_crush.
-  Qed.
-
-  
-  Lemma eqb_refl_true
-    : forall a, eqb a a = true.
-  Proof.
-    intro a.
-    specialize (H0 a a); revert H0.
-    case_match;
-      basic_goal_prep;
-      basic_utils_crush.
-  Qed.
-
-  (* TODO: monitor the effects of this rewrite on performance *)
-  Lemma eqb_ineq_false
-    : forall a b, ((a <> b) \/ (b <> a)) -> eqb a b = false.
-  Proof.
-    intros a b Hneq.
-    specialize (H0 a b); revert H0.
-    case_match;
-      basic_goal_prep;
-      basic_utils_crush.
-  Qed.
-
-  #[export] Instance eqb_boolspec
-    : forall x y : A, BoolSpec (x = y) (x <> y) (eqb x y).
-  Proof.
-    intros.
-    pose proof (eqb_spec x y).
-    destruct (eqb x y); constructor; eauto.
-  Qed.
-  
-  #[local] Hint Rewrite eqb_prop_iff : utils.
-  #[local] Hint Rewrite eqb_refl_true : utils.
-  #[local] Hint Rewrite eqb_ineq_false using (try typeclasses eauto; (left || right); assumption) : utils.
-  
 End __.
 
-Arguments Eqb_ok {A}%type_scope H.
-Arguments eqb_spec {A}%type_scope {Impl Pf} a b.
 Arguments dec {A}%type_scope {DecidableEq} s1 s2.
-   
-#[export] Hint Rewrite eqb_prop_iff using solve[typeclasses eauto] : utils.
-#[export] Hint Rewrite eqb_refl_true using solve[typeclasses eauto] : utils.
+
+  
 (*TODO: also account for _=_->False *)
-#[export] Hint Rewrite eqb_ineq_false using (try typeclasses eauto; (left || right); assumption) : utils.
-
-Ltac eqb_case i j :=
-  pose proof (eqb_spec i j); destruct (eqb i j);[ subst i |].
-
-
-#[export] Instance bool_eqb : Eqb bool := Bool.eqb.
-
-#[export] Instance bool_eqb_ok : Eqb_ok bool_eqb.
-Proof.
-  intros a b.
-  unfold eqb, bool_eqb.
-  destruct (Coq.Bool.Bool.eqb_spec a b); eauto.
-Qed.
-
-(* TODO move code below to specific files *)
-
-#[export] Instance string_Eqb : Eqb string := String.eqb.
-
-#[export] Instance string_Eqb_ok : Eqb_ok string_Eqb.
-Proof.
-  intros a b.
-  unfold eqb, string_Eqb.
-  destruct (String.eqb_spec a b); auto.
-Qed.
-
-
-#[export] Instance nat_eqb : Eqb nat := Nat.eqb.
-
-#[export] Instance nat_eqb_ok : Eqb_ok nat_eqb.
-Proof.
-  intros a b.
-  unfold eqb, nat_eqb.
-  destruct (Decidable.Nat.eqb_spec a b); eauto.
-Qed.
-
-#[export] Instance int_eqb : Eqb int := Uint63.eqb.
-
-#[export] Instance int_eqb_ok : Eqb_ok int_eqb.
-Proof.
-  intros a b.
-  unfold eqb, int_eqb.
-  case_match; [eapply Uint63.eqb_spec| eapply eqb_false_spec]; eauto.
-Qed.
+#[export] Hint Rewrite eqb_ineq_false
+  using (try typeclasses eauto; (left || right); assumption) : bool.
