src/Utils/Options.v
@@ -1,48 +1,10 @@
 Set Implicit Arguments.
 
 From Utils Require Import Base Booleans Eqb Default.
+From coqutil Require Export Option.
 
 Section __.
-  Context (A : Type)
-    `{Eqb_ok A}.  
-
-  Lemma invert_none_some (x : A)
-    : None = Some x <-> False.
-  Proof. prove_inversion_lemma. Qed.
-  Hint Rewrite invert_none_some : utils.
-
-  Lemma invert_some_none (x : A)
-    : Some x = None <-> False.
-  Proof. prove_inversion_lemma. Qed.
-  Hint Rewrite invert_some_none : utils.
-  
-  Lemma invert_some_some (x y : A)
-    : Some x = Some y <-> x = y.
-  Proof. prove_inversion_lemma. Qed.
-  Hint Rewrite invert_some_some : utils.
-
-  #[export] Instance option_eqb : Eqb (option A) :=
-    fun a b =>
-      match a, b with
-      | Some a, Some b => eqb a b
-      | None, None => true
-      | _, _ => false
-      end.
-
-  #[export] Instance option_eqb_ok : Eqb_ok option_eqb.
-  Proof.
-    unfold Eqb_ok, option_eqb, eqb.
-    intros a b;
-      destruct a;
-      destruct b;
-      basic_goal_prep;
-      basic_utils_crush.
-    pose proof (H0 a a0) as H'.
-    unfold eqb in *.
-    revert H'.
-    case_match;
-      basic_utils_crush.
-  Qed.
+  Context (A : Type).
 
   #[export] Instance option_default : WithDefault (option A) := None.
 
@@ -50,7 +12,3 @@ Section __.
   Definition Is_Some (x : option A) := if x then True else False.
 
 End __.
-
-#[export] Hint Rewrite invert_none_some : utils.
-#[export] Hint Rewrite invert_some_none : utils.
-#[export] Hint Rewrite invert_some_some : utils.
